<?xml version="1.0"?>
<rdf:RDF xmlns="https://purl.org/variablereconciliationontology"
     xml:base="https://purl.org/variablereconciliationontology"
     xmlns:dc="http://purl.org/dc/elements/1.1/"
     xmlns:ns="http://creativecommons.org/ns#"
     xmlns:owl="http://www.w3.org/2002/07/owl#"
     xmlns:rdf="http://www.w3.org/1999/02/22-rdf-syntax-ns#"
     xmlns:xml="http://www.w3.org/XML/1998/namespace"
     xmlns:xsd="http://www.w3.org/2001/XMLSchema#"
     xmlns:rdfs="http://www.w3.org/2000/01/rdf-schema#"
     xmlns:vann="http://purl.org/vocab/vann/"
     xmlns:terms="http://purl.org/dc/terms/"
     xmlns:protege="http://protege.stanford.edu/plugins/owl/protege#"
     xmlns:resource="http://semanticscience.org/resource/"
     xmlns:oboe-core="http://ecoinformatics.org/oboe/oboe.1.2/oboe-core.owl#"
     xmlns:oboe-characteristics="http://ecoinformatics.org/oboe/oboe.1.2/oboe-characteristics.owl#"
     xmlns:variablereconciliationontology="https://purl.org/variablereconciliationontology#">
    <owl:Ontology rdf:about="https://purl.org/variablereconciliationontology">
        <owl:imports rdf:resource="http://ecoinformatics.org/oboe/oboe.1.2/oboe.owl"/>
        <owl:imports rdf:resource="http://ontology.cybershare.utep.edu/ELSEWeb/elseweb-data.owl"/>
        <ns:license>https://creativecommons.org/licenses/by-nc-nd/4.0/</ns:license>
        <dc:creator>Raul Alejandro Vargas Acosta (https://github.com/alex-vargas)</dc:creator>
        <dc:description>The Variable Reconciliation Ontology (VaR-O) is designed to capture scientific variables and identify those that are semantically equivalent given their type and scientific assumptions.</dc:description>
        <dc:rights>Free to share, non-commercial use, no derivatives</dc:rights>
        <dc:title>Variable Reconciliation Ontology (VaR-O)</dc:title>
        <terms:modified>2024-04-17</terms:modified>
        <owl:versionInfo rdf:datatype="http://www.w3.org/2001/XMLSchema#decimal">1.0</owl:versionInfo>
    </owl:Ontology>
    


    <!-- 
    ///////////////////////////////////////////////////////////////////////////////////////
    //
    // Object Properties
    //
    ///////////////////////////////////////////////////////////////////////////////////////
     -->

    


    <!-- https://purl.org/variablereconciliationontology#equivalencies -->

    <owl:ObjectProperty rdf:about="https://purl.org/variablereconciliationontology#equivalencies"/>
    


    <!-- 
    ///////////////////////////////////////////////////////////////////////////////////////
    //
    // Data properties
    //
    ///////////////////////////////////////////////////////////////////////////////////////
     -->

    


    <!-- https://purl.org/variablereconciliationontology#NaturalFlow -->

    <owl:DatatypeProperty rdf:about="https://purl.org/variablereconciliationontology#NaturalFlow"/>
    


    <!-- https://purl.org/variablereconciliationontology#RealFlow -->

    <owl:DatatypeProperty rdf:about="https://purl.org/variablereconciliationontology#RealFlow"/>
    


    <!-- https://purl.org/variablereconciliationontology#Scientific-Assumptions -->

    <owl:DatatypeProperty rdf:about="https://purl.org/variablereconciliationontology#Scientific-Assumptions">
        <rdfs:domain rdf:resource="https://purl.org/variablereconciliationontology#ScientificVariable"/>
        <rdfs:comment>This class is the parent class of properties that can describe scientific assumptions.</rdfs:comment>
        <rdfs:label>Scientific-Assumptions</rdfs:label>
    </owl:DatatypeProperty>
    


    <!-- https://purl.org/variablereconciliationontology#abstractRange -->

    <owl:DatatypeProperty rdf:about="https://purl.org/variablereconciliationontology#abstractRange">
        <rdfs:subPropertyOf rdf:resource="https://purl.org/variablereconciliationontology#Scientific-Assumptions"/>
        <rdfs:range rdf:resource="http://www.w3.org/2001/XMLSchema#double"/>
        <rdfs:comment>This property describes a scientific assumption that comprehends a range given in continous data.</rdfs:comment>
        <rdfs:label>abstractRange</rdfs:label>
    </owl:DatatypeProperty>
    


    <!-- https://purl.org/variablereconciliationontology#hasLatitude -->

    <owl:DatatypeProperty rdf:about="https://purl.org/variablereconciliationontology#hasLatitude">
        <rdfs:subPropertyOf rdf:resource="https://purl.org/variablereconciliationontology#Scientific-Assumptions"/>
        <rdfs:range rdf:resource="http://www.w3.org/2001/XMLSchema#double"/>
        <rdfs:comment>This class describes a scientific assumption that represents latitude given in continous data.</rdfs:comment>
        <rdfs:label>hasLatitude</rdfs:label>
    </owl:DatatypeProperty>
    


    <!-- https://purl.org/variablereconciliationontology#hasLongitude -->

    <owl:DatatypeProperty rdf:about="https://purl.org/variablereconciliationontology#hasLongitude">
        <rdfs:subPropertyOf rdf:resource="https://purl.org/variablereconciliationontology#Scientific-Assumptions"/>
        <rdfs:range rdf:resource="http://www.w3.org/2001/XMLSchema#double"/>
        <rdfs:comment>This class describes a scientific assumption that represents longitude given in continous data.</rdfs:comment>
        <rdfs:label>hasLongitude</rdfs:label>
    </owl:DatatypeProperty>
    


    <!-- https://purl.org/variablereconciliationontology#isNaturalFlow -->

    <owl:DatatypeProperty rdf:about="https://purl.org/variablereconciliationontology#isNaturalFlow">
        <rdfs:subPropertyOf rdf:resource="https://purl.org/variablereconciliationontology#Scientific-Assumptions"/>
        <rdfs:range rdf:resource="http://www.w3.org/2001/XMLSchema#string"/>
        <rdfs:comment>This class describes a scientific assumption that represents natural flow of some property (e.g., water)</rdfs:comment>
        <rdfs:label>isNaturalFlow</rdfs:label>
    </owl:DatatypeProperty>
    


    <!-- https://purl.org/variablereconciliationontology#isRealFlow -->

    <owl:DatatypeProperty rdf:about="https://purl.org/variablereconciliationontology#isRealFlow">
        <rdfs:subPropertyOf rdf:resource="https://purl.org/variablereconciliationontology#Scientific-Assumptions"/>
        <rdfs:range rdf:resource="http://www.w3.org/2001/XMLSchema#string"/>
        <rdfs:comment>This class describes a scientific assumption that represents the real flow of some property (e.g., water)</rdfs:comment>
        <rdfs:label>isRealFlow</rdfs:label>
    </owl:DatatypeProperty>
    


    <!-- https://purl.org/variablereconciliationontology#other -->

    <owl:DatatypeProperty rdf:about="https://purl.org/variablereconciliationontology#other"/>
    


    <!-- 
    ///////////////////////////////////////////////////////////////////////////////////////
    //
    // Classes
    //
    ///////////////////////////////////////////////////////////////////////////////////////
     -->

    


    <!-- http://ecoinformatics.org/oboe/oboe.1.2/oboe-characteristics.owl#AmountOfSubstanceConcentration -->

    <owl:Class rdf:about="http://ecoinformatics.org/oboe/oboe.1.2/oboe-characteristics.owl#AmountOfSubstanceConcentration"/>
    


    <!-- http://ecoinformatics.org/oboe/oboe.1.2/oboe-characteristics.owl#Temperature -->

    <owl:Class rdf:about="http://ecoinformatics.org/oboe/oboe.1.2/oboe-characteristics.owl#Temperature"/>
    


    <!-- http://ecoinformatics.org/oboe/oboe.1.2/oboe-core.owl#Entity -->

    <owl:Class rdf:about="http://ecoinformatics.org/oboe/oboe.1.2/oboe-core.owl#Entity"/>
    


    <!-- http://ecoinformatics.org/oboe/oboe.1.2/oboe-core.owl#MeasuredCharacteristic -->

    <owl:Class rdf:about="http://ecoinformatics.org/oboe/oboe.1.2/oboe-core.owl#MeasuredCharacteristic">
        <owl:equivalentClass rdf:resource="https://purl.org/variablereconciliationontology#ScientificVariable"/>
    </owl:Class>
    


    <!-- https://purl.org/variablereconciliationontology#Abstract -->

    <owl:Class rdf:about="https://purl.org/variablereconciliationontology#Abstract">
        <rdfs:subClassOf rdf:resource="https://purl.org/variablereconciliationontology#ScientificVariable"/>
        <rdfs:comment>This class formalizes an example of a classification of a scientific variable. It is used to show how variables can be classified.</rdfs:comment>
        <rdfs:label>Abstract</rdfs:label>
    </owl:Class>
    


    <!-- https://purl.org/variablereconciliationontology#Caballo_Reservoir -->

    <owl:Class rdf:about="https://purl.org/variablereconciliationontology#Caballo_Reservoir">
        <owl:equivalentClass>
            <owl:Class>
                <owl:intersectionOf rdf:parseType="Collection">
                    <owl:Restriction>
                        <owl:onProperty rdf:resource="https://purl.org/variablereconciliationontology#hasLatitude"/>
                        <owl:someValuesFrom>
                            <rdfs:Datatype>
                                <owl:onDatatype rdf:resource="http://www.w3.org/2001/XMLSchema#double"/>
                                <owl:withRestrictions rdf:parseType="Collection">
                                    <rdf:Description>
                                        <xsd:minInclusive rdf:datatype="http://www.w3.org/2001/XMLSchema#double">32.88617</xsd:minInclusive>
                                    </rdf:Description>
                                    <rdf:Description>
                                        <xsd:maxInclusive rdf:datatype="http://www.w3.org/2001/XMLSchema#double">33.01667</xsd:maxInclusive>
                                    </rdf:Description>
                                </owl:withRestrictions>
                            </rdfs:Datatype>
                        </owl:someValuesFrom>
                    </owl:Restriction>
                    <owl:Restriction>
                        <owl:onProperty rdf:resource="https://purl.org/variablereconciliationontology#hasLongitude"/>
                        <owl:someValuesFrom>
                            <rdfs:Datatype>
                                <owl:onDatatype rdf:resource="http://www.w3.org/2001/XMLSchema#double"/>
                                <owl:withRestrictions rdf:parseType="Collection">
                                    <rdf:Description>
                                        <xsd:minInclusive rdf:datatype="http://www.w3.org/2001/XMLSchema#double">-107.32681</xsd:minInclusive>
                                    </rdf:Description>
                                    <rdf:Description>
                                        <xsd:maxInclusive rdf:datatype="http://www.w3.org/2001/XMLSchema#double">-107.27036</xsd:maxInclusive>
                                    </rdf:Description>
                                </owl:withRestrictions>
                            </rdfs:Datatype>
                        </owl:someValuesFrom>
                    </owl:Restriction>
                </owl:intersectionOf>
            </owl:Class>
        </owl:equivalentClass>
        <rdfs:subClassOf rdf:resource="https://purl.org/variablereconciliationontology#New_Mexico"/>
        <rdfs:comment>This class will contain all individuals that satisfy the given condition given their latitude and longitude.</rdfs:comment>
        <rdfs:label>Caballo_Reservoir</rdfs:label>
    </owl:Class>
    


    <!-- https://purl.org/variablereconciliationontology#Elephant_Butte -->

    <owl:Class rdf:about="https://purl.org/variablereconciliationontology#Elephant_Butte">
        <owl:equivalentClass>
            <owl:Class>
                <owl:intersectionOf rdf:parseType="Collection">
                    <owl:Restriction>
                        <owl:onProperty rdf:resource="https://purl.org/variablereconciliationontology#hasLatitude"/>
                        <owl:someValuesFrom>
                            <rdfs:Datatype>
                                <owl:onDatatype rdf:resource="http://www.w3.org/2001/XMLSchema#double"/>
                                <owl:withRestrictions rdf:parseType="Collection">
                                    <rdf:Description>
                                        <xsd:minInclusive rdf:datatype="http://www.w3.org/2001/XMLSchema#double">33.1355</xsd:minInclusive>
                                    </rdf:Description>
                                    <rdf:Description>
                                        <xsd:maxInclusive rdf:datatype="http://www.w3.org/2001/XMLSchema#double">33.34708</xsd:maxInclusive>
                                    </rdf:Description>
                                </owl:withRestrictions>
                            </rdfs:Datatype>
                        </owl:someValuesFrom>
                    </owl:Restriction>
                    <owl:Restriction>
                        <owl:onProperty rdf:resource="https://purl.org/variablereconciliationontology#hasLongitude"/>
                        <owl:someValuesFrom>
                            <rdfs:Datatype>
                                <owl:onDatatype rdf:resource="http://www.w3.org/2001/XMLSchema#double"/>
                                <owl:withRestrictions rdf:parseType="Collection">
                                    <rdf:Description>
                                        <xsd:minInclusive rdf:datatype="http://www.w3.org/2001/XMLSchema#double">-107.26781</xsd:minInclusive>
                                    </rdf:Description>
                                    <rdf:Description>
                                        <xsd:maxInclusive rdf:datatype="http://www.w3.org/2001/XMLSchema#double">-107.13822</xsd:maxInclusive>
                                    </rdf:Description>
                                </owl:withRestrictions>
                            </rdfs:Datatype>
                        </owl:someValuesFrom>
                    </owl:Restriction>
                </owl:intersectionOf>
            </owl:Class>
        </owl:equivalentClass>
        <rdfs:subClassOf rdf:resource="https://purl.org/variablereconciliationontology#New_Mexico"/>
        <rdfs:comment>This class will contain all individuals that satisfy the given condition given their latitude and longitude.</rdfs:comment>
        <rdfs:label>Elephant_Butte</rdfs:label>
    </owl:Class>
    


    <!-- https://purl.org/variablereconciliationontology#Equivalencies -->

    <owl:Class rdf:about="https://purl.org/variablereconciliationontology#Equivalencies">
        <rdfs:subClassOf rdf:resource="https://purl.org/variablereconciliationontology#ScientificVariable"/>
        <rdfs:comment>This class formalizes an example of a classification of a scientific variable. It is used to show how variables can be classified.</rdfs:comment>
        <rdfs:label>Equivalencies</rdfs:label>
    </owl:Class>
    


    <!-- https://purl.org/variablereconciliationontology#Flow -->

    <owl:Class rdf:about="https://purl.org/variablereconciliationontology#Flow">
        <rdfs:subClassOf rdf:resource="https://purl.org/variablereconciliationontology#ScientificVariable"/>
        <rdfs:comment>This class formalizes an example of a classification of a scientific variable. It is used to show how variables can be classified.</rdfs:comment>
        <rdfs:label>Flow</rdfs:label>
    </owl:Class>
    


    <!-- https://purl.org/variablereconciliationontology#Fort_Quitman -->

    <owl:Class rdf:about="https://purl.org/variablereconciliationontology#Fort_Quitman">
        <owl:equivalentClass>
            <owl:Class>
                <owl:intersectionOf rdf:parseType="Collection">
                    <owl:Restriction>
                        <owl:onProperty rdf:resource="https://purl.org/variablereconciliationontology#hasLatitude"/>
                        <owl:someValuesFrom>
                            <rdfs:Datatype>
                                <owl:onDatatype rdf:resource="http://www.w3.org/2001/XMLSchema#double"/>
                                <owl:withRestrictions rdf:parseType="Collection">
                                    <rdf:Description>
                                        <xsd:minInclusive rdf:datatype="http://www.w3.org/2001/XMLSchema#double">31.0482</xsd:minInclusive>
                                    </rdf:Description>
                                    <rdf:Description>
                                        <xsd:maxInclusive rdf:datatype="http://www.w3.org/2001/XMLSchema#double">31.0644</xsd:maxInclusive>
                                    </rdf:Description>
                                </owl:withRestrictions>
                            </rdfs:Datatype>
                        </owl:someValuesFrom>
                    </owl:Restriction>
                    <owl:Restriction>
                        <owl:onProperty rdf:resource="https://purl.org/variablereconciliationontology#hasLongitude"/>
                        <owl:someValuesFrom>
                            <rdfs:Datatype>
                                <owl:onDatatype rdf:resource="http://www.w3.org/2001/XMLSchema#double"/>
                                <owl:withRestrictions rdf:parseType="Collection">
                                    <rdf:Description>
                                        <xsd:minInclusive rdf:datatype="http://www.w3.org/2001/XMLSchema#double">-105.5951</xsd:minInclusive>
                                    </rdf:Description>
                                    <rdf:Description>
                                        <xsd:maxInclusive rdf:datatype="http://www.w3.org/2001/XMLSchema#double">-105.5769</xsd:maxInclusive>
                                    </rdf:Description>
                                </owl:withRestrictions>
                            </rdfs:Datatype>
                        </owl:someValuesFrom>
                    </owl:Restriction>
                </owl:intersectionOf>
            </owl:Class>
        </owl:equivalentClass>
        <rdfs:subClassOf rdf:resource="https://purl.org/variablereconciliationontology#New_Mexico"/>
        <rdfs:comment>This class will contain all individuals that satisfy the given condition given their latitude and longitude.</rdfs:comment>
        <rdfs:label>Fort_Quitman</rdfs:label>
    </owl:Class>
    


    <!-- https://purl.org/variablereconciliationontology#NaturalFlow -->

    <owl:Class rdf:about="https://purl.org/variablereconciliationontology#NaturalFlow">
        <owl:equivalentClass>
            <owl:Class>
                <owl:unionOf rdf:parseType="Collection">
                    <owl:Restriction>
                        <owl:onProperty rdf:resource="https://purl.org/variablereconciliationontology#isNaturalFlow"/>
                        <owl:hasValue>true</owl:hasValue>
                    </owl:Restriction>
                    <owl:Restriction>
                        <owl:onProperty rdf:resource="https://purl.org/variablereconciliationontology#isRealFlow"/>
                        <owl:hasValue>false</owl:hasValue>
                    </owl:Restriction>
                </owl:unionOf>
            </owl:Class>
        </owl:equivalentClass>
        <rdfs:subClassOf rdf:resource="https://purl.org/variablereconciliationontology#Flow"/>
    </owl:Class>
    


    <!-- https://purl.org/variablereconciliationontology#NaturalWaterFlow -->

    <owl:Class rdf:about="https://purl.org/variablereconciliationontology#NaturalWaterFlow">
        <owl:equivalentClass>
            <owl:Class>
                <owl:intersectionOf rdf:parseType="Collection">
                    <rdf:Description rdf:about="https://purl.org/variablereconciliationontology#NaturalFlow"/>
                    <rdf:Description rdf:about="https://purl.org/variablereconciliationontology#WaterFlow"/>
                </owl:intersectionOf>
            </owl:Class>
        </owl:equivalentClass>
        <rdfs:subClassOf rdf:resource="https://purl.org/variablereconciliationontology#Equivalencies"/>
        <rdfs:comment>This class is shown as an example of how equivalency rules can be used to describe a classification of a scientific variable. In this class, all variables (instances) that satisfy the rules specified in &quot;Equivalent To&quot; are going to get categorized as the natural flow of water.</rdfs:comment>
        <rdfs:label>NaturalWaterFlow</rdfs:label>
    </owl:Class>
    


    <!-- https://purl.org/variablereconciliationontology#New_Mexico -->

    <owl:Class rdf:about="https://purl.org/variablereconciliationontology#New_Mexico">
        <rdfs:subClassOf rdf:resource="http://ontology.cybershare.utep.edu/ELSEWeb/elseweb-data.owl#NamedGeographicRegion"/>
        <rdfs:comment>This class represents a named region</rdfs:comment>
        <rdfs:label>New_Mexico</rdfs:label>
    </owl:Class>
    


    <!-- https://purl.org/variablereconciliationontology#Precipitation -->

    <owl:Class rdf:about="https://purl.org/variablereconciliationontology#Precipitation">
        <rdfs:subClassOf rdf:resource="http://ecoinformatics.org/oboe/oboe.1.2/oboe-core.owl#MeasuredCharacteristic"/>
        <rdfs:comment>A measured characteristic of an entity that represents precipitation.</rdfs:comment>
        <rdfs:label>Precipitation</rdfs:label>
    </owl:Class>
    


    <!-- https://purl.org/variablereconciliationontology#Range -->

    <owl:Class rdf:about="https://purl.org/variablereconciliationontology#Range">
        <owl:equivalentClass>
            <owl:Restriction>
                <owl:onProperty rdf:resource="https://purl.org/variablereconciliationontology#abstractRange"/>
                <owl:someValuesFrom>
                    <rdfs:Datatype>
                        <owl:onDatatype rdf:resource="http://www.w3.org/2001/XMLSchema#double"/>
                        <owl:withRestrictions rdf:parseType="Collection">
                            <rdf:Description>
                                <xsd:minInclusive rdf:datatype="http://www.w3.org/2001/XMLSchema#double">72.4</xsd:minInclusive>
                            </rdf:Description>
                            <rdf:Description>
                                <xsd:maxInclusive rdf:datatype="http://www.w3.org/2001/XMLSchema#double">124.42</xsd:maxInclusive>
                            </rdf:Description>
                        </owl:withRestrictions>
                    </rdfs:Datatype>
                </owl:someValuesFrom>
            </owl:Restriction>
        </owl:equivalentClass>
        <rdfs:subClassOf rdf:resource="https://purl.org/variablereconciliationontology#Abstract"/>
        <rdfs:comment>This class depicts an example of how variables can be classified accordingly to a specific range. The range is described in the &quot;Equivalent To&quot; property.</rdfs:comment>
        <rdfs:label>Range</rdfs:label>
    </owl:Class>
    


    <!-- https://purl.org/variablereconciliationontology#RealFlow -->

    <owl:Class rdf:about="https://purl.org/variablereconciliationontology#RealFlow">
        <owl:equivalentClass>
            <owl:Class>
                <owl:unionOf rdf:parseType="Collection">
                    <owl:Restriction>
                        <owl:onProperty rdf:resource="https://purl.org/variablereconciliationontology#isNaturalFlow"/>
                        <owl:hasValue>false</owl:hasValue>
                    </owl:Restriction>
                    <owl:Restriction>
                        <owl:onProperty rdf:resource="https://purl.org/variablereconciliationontology#isRealFlow"/>
                        <owl:hasValue>true</owl:hasValue>
                    </owl:Restriction>
                </owl:unionOf>
            </owl:Class>
        </owl:equivalentClass>
        <rdfs:subClassOf rdf:resource="https://purl.org/variablereconciliationontology#Flow"/>
    </owl:Class>
    


    <!-- https://purl.org/variablereconciliationontology#RealWaterFlow -->

    <owl:Class rdf:about="https://purl.org/variablereconciliationontology#RealWaterFlow">
        <owl:equivalentClass>
            <owl:Class>
                <owl:intersectionOf rdf:parseType="Collection">
                    <rdf:Description rdf:about="https://purl.org/variablereconciliationontology#RealFlow"/>
                    <rdf:Description rdf:about="https://purl.org/variablereconciliationontology#WaterFlow"/>
                </owl:intersectionOf>
            </owl:Class>
        </owl:equivalentClass>
        <rdfs:subClassOf rdf:resource="https://purl.org/variablereconciliationontology#Equivalencies"/>
        <rdfs:comment>This class is shown as an example of how equivalency rules can be used to describe a classification of a scientific variable. In this class, all variables (instances) that satisfy the rules specified in &quot;Equivalent To&quot; are going to get categorized as the real flow of water.</rdfs:comment>
        <rdfs:label>RealWaterFlow</rdfs:label>
    </owl:Class>
    


    <!-- https://purl.org/variablereconciliationontology#RunOff -->

    <owl:Class rdf:about="https://purl.org/variablereconciliationontology#RunOff">
        <rdfs:subClassOf rdf:resource="http://ecoinformatics.org/oboe/oboe.1.2/oboe-core.owl#MeasuredCharacteristic"/>
        <rdfs:comment>A measured characteristic of an entity that represents runoff</rdfs:comment>
        <rdfs:label>RunOff</rdfs:label>
    </owl:Class>
    


    <!-- https://purl.org/variablereconciliationontology#San_Marcial -->

    <owl:Class rdf:about="https://purl.org/variablereconciliationontology#San_Marcial">
        <owl:equivalentClass>
            <owl:Class>
                <owl:intersectionOf rdf:parseType="Collection">
                    <owl:Restriction>
                        <owl:onProperty rdf:resource="https://purl.org/variablereconciliationontology#hasLatitude"/>
                        <owl:someValuesFrom>
                            <rdfs:Datatype>
                                <owl:onDatatype rdf:resource="http://www.w3.org/2001/XMLSchema#double"/>
                                <owl:withRestrictions rdf:parseType="Collection">
                                    <rdf:Description>
                                        <xsd:minInclusive rdf:datatype="http://www.w3.org/2001/XMLSchema#double">33.581015</xsd:minInclusive>
                                    </rdf:Description>
                                    <rdf:Description>
                                        <xsd:maxInclusive rdf:datatype="http://www.w3.org/2001/XMLSchema#double">33.751051</xsd:maxInclusive>
                                    </rdf:Description>
                                </owl:withRestrictions>
                            </rdfs:Datatype>
                        </owl:someValuesFrom>
                    </owl:Restriction>
                    <owl:Restriction>
                        <owl:onProperty rdf:resource="https://purl.org/variablereconciliationontology#hasLongitude"/>
                        <owl:someValuesFrom>
                            <rdfs:Datatype>
                                <owl:onDatatype rdf:resource="http://www.w3.org/2001/XMLSchema#double"/>
                                <owl:withRestrictions rdf:parseType="Collection">
                                    <rdf:Description>
                                        <xsd:minInclusive rdf:datatype="http://www.w3.org/2001/XMLSchema#double">-107.10517</xsd:minInclusive>
                                    </rdf:Description>
                                    <rdf:Description>
                                        <xsd:maxInclusive rdf:datatype="http://www.w3.org/2001/XMLSchema#double">-106.938907</xsd:maxInclusive>
                                    </rdf:Description>
                                </owl:withRestrictions>
                            </rdfs:Datatype>
                        </owl:someValuesFrom>
                    </owl:Restriction>
                </owl:intersectionOf>
            </owl:Class>
        </owl:equivalentClass>
        <rdfs:subClassOf rdf:resource="https://purl.org/variablereconciliationontology#New_Mexico"/>
        <rdfs:comment>This class will contain all individuals that satisfy the given condition given their latitude and longitude.</rdfs:comment>
        <rdfs:label>San_Marcial</rdfs:label>
    </owl:Class>
    


    <!-- https://purl.org/variablereconciliationontology#ScientificVariable -->

    <owl:Class rdf:about="https://purl.org/variablereconciliationontology#ScientificVariable">
        <rdfs:comment>This class represents the &quot;Scientific Variable&quot; that can be represented in the ontology. This includes &quot;Water Flow&quot;, and others. Each variable has properties that represent scientific assumptions.</rdfs:comment>
        <rdfs:label>ScientificVariable</rdfs:label>
    </owl:Class>
    


    <!-- https://purl.org/variablereconciliationontology#WaterFlow -->

    <owl:Class rdf:about="https://purl.org/variablereconciliationontology#WaterFlow">
        <rdfs:subClassOf rdf:resource="https://purl.org/variablereconciliationontology#ScientificVariable"/>
        <rdfs:comment>This class is shown as an example of how equivalency rules can be used to describe a classification of a scientific variable. In this class all variables are classified as the flow of water in a region.</rdfs:comment>
        <rdfs:label>WaterFlow</rdfs:label>
    </owl:Class>
    


    <!-- https://purl.org/variablereconciliationontology#WaterPrice -->

    <owl:Class rdf:about="https://purl.org/variablereconciliationontology#WaterPrice">
        <rdfs:subClassOf rdf:resource="http://ecoinformatics.org/oboe/oboe.1.2/oboe-core.owl#MeasuredCharacteristic"/>
        <rdfs:comment>A measured characteristic of an entity that represents the price of water.</rdfs:comment>
        <rdfs:label>WaterPrice</rdfs:label>
    </owl:Class>
    


    <!-- 
    ///////////////////////////////////////////////////////////////////////////////////////
    //
    // Annotations
    //
    ///////////////////////////////////////////////////////////////////////////////////////
     -->

    <rdf:Description rdf:about="https://purl.org/variablereconciliationontology#NaturalFlow">
        <rdfs:label>NaturalFlow</rdfs:label>
        <rdfs:comment>This class is shown as an example of how equivalency rules can be used to describe a classification of a scientific variable. In this class, all variables (instances) that satisfy the rules specified in &quot;Equivalent To&quot; are going to get categorized as the natural flow of something. Notice that this is not specific to water.</rdfs:comment>
    </rdf:Description>
    <rdf:Description rdf:about="https://purl.org/variablereconciliationontology#RealFlow">
        <rdfs:comment>This class is shown as an example of how equivalency rules can be used to describe a classification of a scientific variable. In this class, all variables (instances) that satisfy the rules specified in &quot;Equivalent To&quot; are going to get categorized as the real flow of something. Notice that this is not specific to water.</rdfs:comment>
        <rdfs:label>RealFlow</rdfs:label>
    </rdf:Description>
</rdf:RDF>



<!-- Generated by the OWL API (version 4.5.9.2019-02-01T07:24:44Z) https://github.com/owlcs/owlapi -->

